extend lib_list in src/: 4 lists

src/ArrayList.fst
@@ -14,268 +14,304 @@ module FS = FStar.FiniteSet.Base
 module AL = ArrayListGen
 
 let read_in_place
-  (#pred1 #pred2 #pred3: status -> prop)
+  (#pred1 #pred2 #pred3 #pred4: status -> prop)
   (r:A.array cell)
-  (hd1 hd2 hd3:Ghost.erased nat)
+  (hd1 hd2 hd3 hd4:Ghost.erased nat)
   (idx:US.t{US.v idx < A.length r})
   : Steel status
-          (varraylist pred1 pred2 pred3 r hd1 hd2 hd3)
-          (fun _ -> varraylist pred1 pred2 pred3 r hd1 hd2 hd3)
+          (varraylist pred1 pred2 pred3 pred4 r hd1 hd2 hd3 hd4)
+          (fun _ -> varraylist pred1 pred2 pred3 pred4 r hd1 hd2 hd3 hd4)
           (requires fun _ -> True)
           (ensures fun h0 result h1 ->
-            result == AL.get_data (Seq.index (v_arraylist pred1 pred2 pred3 r hd1 hd2 hd3 h0) (US.v idx)) /\
-            h0 (varraylist pred1 pred2 pred3 r hd1 hd2 hd3) ==
-            h1 (varraylist pred1 pred2 pred3 r hd1 hd2 hd3))
-  = AL.read_in_place r hd1 hd2 hd3 idx
+            result == AL.get_data (Seq.index (v_arraylist pred1 pred2 pred3 pred4 r hd1 hd2 hd3 hd4 h0) (US.v idx)) /\
+            h0 (varraylist pred1 pred2 pred3 pred4 r hd1 hd2 hd3 hd4) ==
+            h1 (varraylist pred1 pred2 pred3 pred4 r hd1 hd2 hd3 hd4))
+  = AL.read_in_place r hd1 hd2 hd3 hd4 idx
 
 /// Removes the element at offset [idx] from the dlist pointed to by [hd1]
 let remove
-  (#pred1 #pred2 #pred3: status -> prop)
+  (#pred1 #pred2 #pred3 #pred4: status -> prop)
   (r:A.array cell)
   (hd1:US.t)
-  (hd2 hd3:Ghost.erased nat)
+  (hd2 hd3 hd4:Ghost.erased nat)
   (idx:US.t{US.v idx < A.length r})
    : Steel US.t
-          (varraylist pred1 pred2 pred3 r (US.v hd1) hd2 hd3)
-          (fun hd' -> varraylist pred1 pred2 pred3 r (US.v hd') hd2 hd3)
-          (requires fun h -> AL.mem (US.v idx) (US.v hd1) (h (varraylist pred1 pred2 pred3 r (US.v hd1) hd2 hd3)))
+          (varraylist pred1 pred2 pred3 pred4 r (US.v hd1) hd2 hd3 hd4)
+          (fun hd' -> varraylist pred1 pred2 pred3 pred4 r (US.v hd') hd2 hd3 hd4)
+          (requires fun h -> AL.mem (US.v idx) (US.v hd1) (h (varraylist pred1 pred2 pred3 pred4 r (US.v hd1) hd2 hd3 hd4)))
           (ensures fun h0 hd' h1 ->
-            AL.ptrs_in (US.v hd') (h1 (varraylist pred1 pred2 pred3 r (US.v hd') hd2 hd3)) ==
-            FS.remove (US.v idx) (AL.ptrs_in (US.v hd1) (h0 (varraylist pred1 pred2 pred3 r (US.v hd1) hd2 hd3))) /\
-            AL.ptrs_in hd2 (h1 (varraylist pred1 pred2 pred3 r (US.v hd') hd2 hd3)) ==
-            AL.ptrs_in hd2 (h0 (varraylist pred1 pred2 pred3 r (US.v hd1) hd2 hd3)) /\
-            AL.ptrs_in hd3 (h1 (varraylist pred1 pred2 pred3 r (US.v hd') hd2 hd3)) ==
-            AL.ptrs_in hd3 (h0 (varraylist pred1 pred2 pred3 r (US.v hd1) hd2 hd3)) /\
-            (~ (AL.mem_all (US.v idx) (US.v hd') hd2 hd3 (h1 (varraylist pred1 pred2 pred3 r (US.v hd') hd2 hd3)))) /\
-            AL.dataify (h1 (varraylist pred1 pred2 pred3 r (US.v hd') hd2 hd3)) ==
-            AL.dataify (h0 (varraylist pred1 pred2 pred3 r (US.v hd1) hd2 hd3))
-          )
-  = AL.remove r hd1 hd2 hd3 idx
-
-/// Removes the element at offset [idx] from the dlist pointed to by [hd1]
-inline_for_extraction noextract
-let remove1
-  (#pred1 #pred2 #pred3: status -> prop)
-  (r:A.array cell)
-  (hd1:US.t)
-  (hd2 hd3:Ghost.erased nat)
-  (idx:US.t{US.v idx < A.length r})
-   : Steel US.t
-          (varraylist pred1 pred2 pred3 r (US.v hd1) hd2 hd3)
-          (fun hd' -> varraylist pred1 pred2 pred3 r (US.v hd') hd2 hd3)
-          (requires fun h -> AL.mem (US.v idx) (US.v hd1) (h (varraylist pred1 pred2 pred3 r (US.v hd1) hd2 hd3)))
-          (ensures fun h0 hd' h1 ->
-            let gs0 = h0 (varraylist pred1 pred2 pred3 r (US.v hd1) hd2 hd3) in
-            let gs1 = h1 (varraylist pred1 pred2 pred3 r (US.v hd') hd2 hd3) in
+            let gs0 = h0 (varraylist pred1 pred2 pred3 pred4 r (US.v hd1) hd2 hd3 hd4) in
+            let gs1 = h1 (varraylist pred1 pred2 pred3 pred4 r (US.v hd') hd2 hd3 hd4) in
             AL.ptrs_in (US.v hd') gs1 ==
             FS.remove (US.v idx) (AL.ptrs_in (US.v hd1) gs0) /\
             AL.ptrs_in hd2 gs1 == AL.ptrs_in hd2 gs0 /\
             AL.ptrs_in hd3 gs1 == AL.ptrs_in hd3 gs0 /\
-            (~ (AL.mem_all (US.v idx) (US.v hd') hd2 hd3 gs1)) /\
+            AL.ptrs_in hd4 gs1 == AL.ptrs_in hd4 gs0 /\
+            (~ (AL.mem_all (US.v idx) (US.v hd') hd2 hd3 hd4 gs1)) /\
             AL.dataify gs1 == AL.dataify gs0
           )
-  = remove r hd1 hd2 hd3 idx
+  = AL.remove r hd1 hd2 hd3 hd4 idx
+
+/// Removes the element at offset [idx] from the dlist pointed to by [hd1]
+inline_for_extraction noextract
+let remove1
+  (#pred1 #pred2 #pred3 #pred4: status -> prop)
+  (r:A.array cell)
+  (hd1:US.t)
+  (hd2 hd3 hd4:Ghost.erased nat)
+  (idx:US.t{US.v idx < A.length r})
+   : Steel US.t
+          (varraylist pred1 pred2 pred3 pred4 r (US.v hd1) hd2 hd3 hd4)
+          (fun hd' -> varraylist pred1 pred2 pred3 pred4 r (US.v hd') hd2 hd3 hd4)
+          (requires fun h -> AL.mem (US.v idx) (US.v hd1) (h (varraylist pred1 pred2 pred3 pred4 r (US.v hd1) hd2 hd3 hd4)))
+          (ensures fun h0 hd' h1 ->
+            let gs0 = h0 (varraylist pred1 pred2 pred3 pred4 r (US.v hd1) hd2 hd3 hd4) in
+            let gs1 = h1 (varraylist pred1 pred2 pred3 pred4 r (US.v hd') hd2 hd3 hd4) in
+            AL.ptrs_in (US.v hd') gs1 ==
+            FS.remove (US.v idx) (AL.ptrs_in (US.v hd1) gs0) /\
+            AL.ptrs_in hd2 gs1 == AL.ptrs_in hd2 gs0 /\
+            AL.ptrs_in hd3 gs1 == AL.ptrs_in hd3 gs0 /\
+            AL.ptrs_in hd4 gs1 == AL.ptrs_in hd4 gs0 /\
+            (~ (AL.mem_all (US.v idx) (US.v hd') hd2 hd3 hd4 gs1)) /\
+            AL.dataify gs1 == AL.dataify gs0
+          )
+  = remove r hd1 hd2 hd3 hd4 idx
 
 inline_for_extraction noextract
 let remove2
-  (#pred1 #pred2 #pred3: status -> prop)
+  (#pred1 #pred2 #pred3 #pred4: status -> prop)
   (r:A.array cell)
   (hd1:Ghost.erased nat)
   (hd2:US.t)
-  (hd3:Ghost.erased nat)
+  (hd3 hd4:Ghost.erased nat)
   (idx:US.t{US.v idx < A.length r})
    : Steel US.t
-          (varraylist pred1 pred2 pred3 r hd1 (US.v hd2) hd3)
-          (fun hd' -> varraylist pred1 pred2 pred3 r hd1 (US.v hd') hd3)
-          (requires fun h -> AL.mem (US.v idx) (US.v hd2) (h (varraylist pred1 pred2 pred3 r hd1 (US.v hd2) hd3)))
+          (varraylist pred1 pred2 pred3 pred4 r hd1 (US.v hd2) hd3 hd4)
+          (fun hd' -> varraylist pred1 pred2 pred3 pred4 r hd1 (US.v hd') hd3 hd4)
+          (requires fun h -> AL.mem (US.v idx) (US.v hd2) (h (varraylist pred1 pred2 pred3 pred4 r hd1 (US.v hd2) hd3 hd4)))
           (ensures fun h0 hd' h1 ->
-            let gs0 = h0 (varraylist pred1 pred2 pred3 r hd1 (US.v hd2) hd3) in
-            let gs1 = h1 (varraylist pred1 pred2 pred3 r hd1 (US.v hd') hd3) in
+            let gs0 = h0 (varraylist pred1 pred2 pred3 pred4 r hd1 (US.v hd2) hd3 hd4) in
+            let gs1 = h1 (varraylist pred1 pred2 pred3 pred4 r hd1 (US.v hd') hd3 hd4) in
             AL.ptrs_in (US.v hd') gs1 ==
             FS.remove (US.v idx) (AL.ptrs_in (US.v hd2) gs0) /\
             AL.ptrs_in hd1 gs1 == AL.ptrs_in hd1 gs0 /\
             AL.ptrs_in hd3 gs1 == AL.ptrs_in hd3 gs0 /\
-            (~ (AL.mem_all (US.v idx) hd1 (US.v hd') hd3 gs1)) /\
+            AL.ptrs_in hd4 gs1 == AL.ptrs_in hd4 gs0 /\
+            (~ (AL.mem_all (US.v idx) hd1 (US.v hd') hd3 hd4 gs1)) /\
             AL.dataify gs1 == AL.dataify gs0
           )
-  = AL.permute12 pred1 pred2 pred3 r hd1 (US.v hd2) hd3;
-    let v = remove r hd2 hd1 hd3 idx in
-    AL.permute12 pred2 pred1 pred3 r (US.v v) hd1 hd3;
+  = AL.permute12 pred1 pred2 pred3 pred4 r hd1 (US.v hd2) hd3 hd4;
+    let v = remove r hd2 hd1 hd3 hd4 idx in
+    AL.permute12 pred2 pred1 pred3 pred4 r (US.v v) hd1 hd3 hd4;
     return v
 
 inline_for_extraction noextract
 let remove3
-  (#pred1 #pred2 #pred3: status -> prop)
+  (#pred1 #pred2 #pred3 #pred4: status -> prop)
   (r:A.array cell)
   (hd1:Ghost.erased nat)
   (hd2:Ghost.erased nat)
   (hd3:US.t)
+  (hd4:Ghost.erased nat)
   (idx:US.t{US.v idx < A.length r})
    : Steel US.t
-          (varraylist pred1 pred2 pred3 r hd1 hd2 (US.v hd3))
-          (fun hd' -> varraylist pred1 pred2 pred3 r hd1 hd2 (US.v hd'))
-          (requires fun h -> AL.mem (US.v idx) (US.v hd3) (h (varraylist pred1 pred2 pred3 r hd1 hd2 (US.v hd3))))
+          (varraylist pred1 pred2 pred3 pred4 r hd1 hd2 (US.v hd3) hd4)
+          (fun hd' -> varraylist pred1 pred2 pred3 pred4 r hd1 hd2 (US.v hd') hd4)
+          (requires fun h -> AL.mem (US.v idx) (US.v hd3) (h (varraylist pred1 pred2 pred3 pred4 r hd1 hd2 (US.v hd3) hd4)))
           (ensures fun h0 hd' h1 ->
-            let gs0 = h0 (varraylist pred1 pred2 pred3 r hd1 hd2 (US.v hd3)) in
-            let gs1 = h1 (varraylist pred1 pred2 pred3 r hd1 hd2 (US.v hd')) in
+            let gs0 = h0 (varraylist pred1 pred2 pred3 pred4 r hd1 hd2 (US.v hd3) hd4) in
+            let gs1 = h1 (varraylist pred1 pred2 pred3 pred4 r hd1 hd2 (US.v hd') hd4) in
             AL.ptrs_in (US.v hd') gs1 ==
             FS.remove (US.v idx) (AL.ptrs_in (US.v hd3) gs0) /\
             AL.ptrs_in hd1 gs1 == AL.ptrs_in hd1 gs0 /\
             AL.ptrs_in hd2 gs1 == AL.ptrs_in hd2 gs0 /\
-            (~ (AL.mem_all (US.v idx) hd1 hd2 (US.v hd') gs1)) /\
+            AL.ptrs_in hd4 gs1 == AL.ptrs_in hd4 gs0 /\
+            (~ (AL.mem_all (US.v idx) hd1 hd2 (US.v hd') hd4 gs1)) /\
             AL.dataify gs1 == AL.dataify gs0
           )
-  = AL.permute13 pred1 pred2 pred3 r hd1 hd2 (US.v hd3);
-    let v = remove r hd3 hd2 hd1 idx in
-    AL.permute13 pred3 pred2 pred1 r (US.v v) hd2 hd1;
+  = AL.permute13 pred1 pred2 pred3 pred4 r hd1 hd2 (US.v hd3) hd4;
+    let v = remove r hd3 hd2 hd1 hd4 idx in
+    AL.permute13 pred3 pred2 pred1 pred4 r (US.v v) hd2 hd1 hd4;
     return v
 
 let insert
-  (#pred1 #pred2 #pred3: status -> prop)
+  (#pred1 #pred2 #pred3 #pred4: status -> prop)
   (r:A.array cell)
   (hd:US.t)
-  (hd2 hd3:Ghost.erased nat)
+  (hd2 hd3 hd4:Ghost.erased nat)
   (idx:US.t{idx <> null_ptr /\ US.v idx < A.length r})
   (v: status)
    : Steel unit
-          (varraylist pred1 pred2 pred3 r (US.v hd) hd2 hd3)
-          (fun _ -> varraylist pred1 pred2 pred3 r (US.v idx) hd2 hd3)
-
+          (varraylist pred1 pred2 pred3 pred4 r (US.v hd) hd2 hd3 hd4)
+          (fun _ -> varraylist pred1 pred2 pred3 pred4 r (US.v idx) hd2 hd3 hd4)
           (requires fun h -> pred1 v /\
-            (~ (AL.mem_all (US.v idx) (US.v hd) hd2 hd3 (h (varraylist pred1 pred2 pred3 r (US.v hd) hd2 hd3)))))
-          (ensures fun h0 hd' h1 ->
-            let gs0 = h0 (varraylist pred1 pred2 pred3 r (US.v hd) hd2 hd3) in
-            let gs1 = h1 (varraylist pred1 pred2 pred3 r (US.v idx) hd2 hd3) in
+            (~ (AL.mem_all (US.v idx) (US.v hd) hd2 hd3 hd4 (h (varraylist pred1 pred2 pred3 pred4 r (US.v hd) hd2 hd3 hd4)))))
+          (ensures fun h0 _ h1 ->
+            let gs0 = h0 (varraylist pred1 pred2 pred3 pred4 r (US.v hd) hd2 hd3 hd4) in
+            let gs1 = h1 (varraylist pred1 pred2 pred3 pred4 r (US.v idx) hd2 hd3 hd4) in
             AL.ptrs_in (US.v idx) gs1 ==
             FS.insert (US.v idx) (AL.ptrs_in (US.v hd) gs0) /\
             AL.ptrs_in hd2 gs1 == AL.ptrs_in hd2 gs0 /\
             AL.ptrs_in hd3 gs1 == AL.ptrs_in hd3 gs0 /\
+            AL.ptrs_in hd4 gs1 == AL.ptrs_in hd4 gs0 /\
             AL.dataify gs1 == Seq.upd (AL.dataify gs0) (US.v idx) v
           )
-  = AL.insert r hd hd2 hd3 idx v
+  = AL.insert r hd hd2 hd3 hd4 idx v
 
 let insert1
-  (#pred1 #pred2 #pred3: status -> prop)
+  (#pred1 #pred2 #pred3 #pred4: status -> prop)
   (r:A.array cell)
   (hd:US.t)
-  (hd2 hd3:Ghost.erased nat)
+  (hd2 hd3 hd4:Ghost.erased nat)
   (idx:US.t{idx <> null_ptr /\ US.v idx < A.length r})
   (v: status)
    : Steel unit
-          (varraylist pred1 pred2 pred3 r (US.v hd) hd2 hd3)
-          (fun _ -> varraylist pred1 pred2 pred3 r (US.v idx) hd2 hd3)
+          (varraylist pred1 pred2 pred3 pred4 r (US.v hd) hd2 hd3 hd4)
+          (fun _ -> varraylist pred1 pred2 pred3 pred4 r (US.v idx) hd2 hd3 hd4)
           (requires fun h -> pred1 v /\
-            (~ (AL.mem_all (US.v idx) (US.v hd) hd2 hd3 (h (varraylist pred1 pred2 pred3 r (US.v hd) hd2 hd3)))))
-          (ensures fun h0 hd' h1 ->
-            let gs0 = h0 (varraylist pred1 pred2 pred3 r (US.v hd) hd2 hd3) in
-            let gs1 = h1 (varraylist pred1 pred2 pred3 r (US.v idx) hd2 hd3) in
+            (~ (AL.mem_all (US.v idx) (US.v hd) hd2 hd3 hd4 (h (varraylist pred1 pred2 pred3 pred4 r (US.v hd) hd2 hd3 hd4)))))
+          (ensures fun h0 _ h1 ->
+            let gs0 = h0 (varraylist pred1 pred2 pred3 pred4 r (US.v hd) hd2 hd3 hd4) in
+            let gs1 = h1 (varraylist pred1 pred2 pred3 pred4 r (US.v idx) hd2 hd3 hd4) in
             AL.ptrs_in (US.v idx) gs1 ==
             FS.insert (US.v idx) (AL.ptrs_in (US.v hd) gs0) /\
             AL.ptrs_in hd2 gs1 == AL.ptrs_in hd2 gs0 /\
             AL.ptrs_in hd3 gs1 == AL.ptrs_in hd3 gs0 /\
+            AL.ptrs_in hd4 gs1 == AL.ptrs_in hd4 gs0 /\
             AL.dataify gs1 == Seq.upd (AL.dataify gs0) (US.v idx) v
           )
-  = insert r hd hd2 hd3 idx v
+  = insert r hd hd2 hd3 hd4 idx v
 
 let insert2
-  (#pred1 #pred2 #pred3: status -> prop)
+  (#pred1 #pred2 #pred3 #pred4: status -> prop)
   (r:A.array cell)
   (hd:US.t)
-  (hd1 hd3:Ghost.erased nat)
+  (hd1 hd3 hd4:Ghost.erased nat)
   (idx:US.t{idx <> null_ptr /\ US.v idx < A.length r})
   (v: status)
    : Steel unit
-          (varraylist pred1 pred2 pred3 r hd1 (US.v hd) hd3)
-          (fun _ -> varraylist pred1 pred2 pred3 r hd1 (US.v idx) hd3)
+          (varraylist pred1 pred2 pred3 pred4 r hd1 (US.v hd) hd3 hd4)
+          (fun _ -> varraylist pred1 pred2 pred3 pred4 r hd1 (US.v idx) hd3 hd4)
           (requires fun h -> pred2 v /\
-            (~ (AL.mem_all (US.v idx) hd1 (US.v hd) hd3 (h (varraylist pred1 pred2 pred3 r hd1 (US.v hd) hd3)))))
-          (ensures fun h0 hd' h1 ->
-            let gs0 = h0 (varraylist pred1 pred2 pred3 r hd1 (US.v hd) hd3) in
-            let gs1 = h1 (varraylist pred1 pred2 pred3 r hd1 (US.v idx) hd3) in
+            (~ (AL.mem_all (US.v idx) hd1 (US.v hd) hd3 hd4 (h (varraylist pred1 pred2 pred3 pred4 r hd1 (US.v hd) hd3 hd4)))))
+          (ensures fun h0 _ h1 ->
+            let gs0 = h0 (varraylist pred1 pred2 pred3 pred4 r hd1 (US.v hd) hd3 hd4) in
+            let gs1 = h1 (varraylist pred1 pred2 pred3 pred4 r hd1 (US.v idx) hd3 hd4) in
             AL.ptrs_in (US.v idx) gs1 ==
             FS.insert (US.v idx) (AL.ptrs_in (US.v hd) gs0) /\
             AL.ptrs_in hd1 gs1 == AL.ptrs_in hd1 gs0 /\
             AL.ptrs_in hd3 gs1 == AL.ptrs_in hd3 gs0 /\
+            AL.ptrs_in hd4 gs1 == AL.ptrs_in hd4 gs0 /\
             AL.dataify gs1 == Seq.upd (AL.dataify gs0) (US.v idx) v
           )
-  = AL.permute12 pred1 pred2 pred3 r hd1 (US.v hd) hd3;
-    insert r hd hd1 hd3 idx v;
-    AL.permute12 pred2 pred1 pred3 r (US.v idx) hd1 hd3
+  = AL.permute12 pred1 pred2 pred3 pred4 r hd1 (US.v hd) hd3 hd4;
+    insert r hd hd1 hd3 hd4 idx v;
+    AL.permute12 pred2 pred1 pred3 pred4 r (US.v idx) hd1 hd3 hd4
 
 let insert3
-  (#pred1 #pred2 #pred3: status -> prop)
+  (#pred1 #pred2 #pred3 #pred4: status -> prop)
   (r:A.array cell)
   (hd:US.t)
-  (hd1 hd2:Ghost.erased nat)
+  (hd1 hd2 hd4:Ghost.erased nat)
   (idx:US.t{idx <> null_ptr /\ US.v idx < A.length r})
   (v: status)
    : Steel unit
-          (varraylist pred1 pred2 pred3 r hd1 hd2 (US.v hd))
-          (fun _ -> varraylist pred1 pred2 pred3 r hd1 hd2 (US.v idx))
+          (varraylist pred1 pred2 pred3 pred4 r hd1 hd2 (US.v hd) hd4)
+          (fun _ -> varraylist pred1 pred2 pred3 pred4 r hd1 hd2 (US.v idx) hd4)
           (requires fun h -> pred3 v /\
-            (~ (AL.mem_all (US.v idx) hd1 hd2 (US.v hd) (h (varraylist pred1 pred2 pred3 r hd1 hd2 (US.v hd))))))
-          (ensures fun h0 hd' h1 ->
-            let gs0 = h0 (varraylist pred1 pred2 pred3 r hd1 hd2 (US.v hd)) in
-            let gs1 = h1 (varraylist pred1 pred2 pred3 r hd1 hd2 (US.v idx)) in
+            (~ (AL.mem_all (US.v idx) hd1 hd2 (US.v hd) hd4 (h (varraylist pred1 pred2 pred3 pred4 r hd1 hd2 (US.v hd) hd4)))))
+          (ensures fun h0 _ h1 ->
+            let gs0 = h0 (varraylist pred1 pred2 pred3 pred4 r hd1 hd2 (US.v hd) hd4) in
+            let gs1 = h1 (varraylist pred1 pred2 pred3 pred4 r hd1 hd2 (US.v idx) hd4) in
             AL.ptrs_in (US.v idx) gs1 ==
             FS.insert (US.v idx) (AL.ptrs_in (US.v hd) gs0) /\
             AL.ptrs_in hd1 gs1 == AL.ptrs_in hd1 gs0 /\
             AL.ptrs_in hd2 gs1 == AL.ptrs_in hd2 gs0 /\
+            AL.ptrs_in hd4 gs1 == AL.ptrs_in hd4 gs0 /\
             AL.dataify gs1 == Seq.upd (AL.dataify gs0) (US.v idx) v
           )
-  = AL.permute13 pred1 pred2 pred3 r hd1 hd2 (US.v hd);
-    insert r hd hd2 hd1 idx v;
-    AL.permute13 pred3 pred2 pred1 r (US.v idx) hd2 hd1
+  = AL.permute13 pred1 pred2 pred3 pred4 r hd1 hd2 (US.v hd) hd4;
+    insert r hd hd2 hd1 hd4 idx v;
+    AL.permute13 pred3 pred2 pred1 pred4 r (US.v idx) hd2 hd1 hd4
+
+let insert4
+  (#pred1 #pred2 #pred3 #pred4: status -> prop)
+  (r:A.array cell)
+  (hd:US.t)
+  (hd1 hd2 hd3:Ghost.erased nat)
+  (idx:US.t{idx <> null_ptr /\ US.v idx < A.length r})
+  (v: status)
+   : Steel unit
+          (varraylist pred1 pred2 pred3 pred4 r hd1 hd2 hd3 (US.v hd))
+          (fun _ -> varraylist pred1 pred2 pred3 pred4 r hd1 hd2 hd3 (US.v idx))
+          (requires fun h -> pred4 v /\
+            (~ (AL.mem_all (US.v idx) hd1 hd2 hd3 (US.v hd) (h (varraylist pred1 pred2 pred3 pred4 r hd1 hd2 hd3 (US.v hd))))))
+          (ensures fun h0 _ h1 ->
+            let gs0 = h0 (varraylist pred1 pred2 pred3 pred4 r hd1 hd2 hd3 (US.v hd)) in
+            let gs1 = h1 (varraylist pred1 pred2 pred3 pred4 r hd1 hd2 hd3 (US.v idx)) in
+            AL.ptrs_in (US.v idx) gs1 ==
+            FS.insert (US.v idx) (AL.ptrs_in (US.v hd) gs0) /\
+            AL.ptrs_in hd1 gs1 == AL.ptrs_in hd1 gs0 /\
+            AL.ptrs_in hd2 gs1 == AL.ptrs_in hd2 gs0 /\
+            AL.ptrs_in hd3 gs1 == AL.ptrs_in hd3 gs0 /\
+            AL.dataify gs1 == Seq.upd (AL.dataify gs0) (US.v idx) v
+          )
+  =
+  AL.permute14 pred1 pred2 pred3 pred4 r hd1 hd2 hd3 (US.v hd);
+  insert r hd hd2 hd3 hd1 idx v;
+  AL.permute14 pred4 pred2 pred3 pred1 r (US.v idx) hd2 hd3 hd1
 
 let extend
-  (#pred1 #pred2 #pred3: status -> prop)
+  (#pred1 #pred2 #pred3 #pred4: status -> prop)
   (r:A.array cell)
   (hd:US.t{hd == null_ptr \/ US.v hd < A.length r})
-  (hd2 hd3:Ghost.erased nat)
+  (hd2 hd3 hd4:Ghost.erased nat)
   (k:US.t{US.v k + 1 <= A.length r /\ US.fits (US.v k + 1)})
   (v: status)
   : Steel unit
-          (AL.varraylist pred1 pred2 pred3 (A.split_l r k) (US.v hd) hd2 hd3 `star`
+          (AL.varraylist pred1 pred2 pred3 pred4 (A.split_l r k) (US.v hd) hd2 hd3 hd4 `star`
             A.varray (A.split_l (A.split_r r k) 1sz))
           (fun _ ->
-            AL.varraylist pred1 pred2 pred3 (A.split_l r (k `US.add` 1sz)) (US.v k) hd2 hd3)
+            AL.varraylist pred1 pred2 pred3 pred4 (A.split_l r (k `US.add` 1sz)) (US.v k) hd2 hd3 hd4)
           (requires fun _ ->
             k <> null_ptr /\ pred1 v)
           (ensures fun h0 _ h1 ->
             A.length_fits r;
-            let gs0 = h0 (varraylist pred1 pred2 pred3 (A.split_l r k) (US.v hd) hd2 hd3) in
-            let gs1 = h1 (varraylist pred1 pred2 pred3 (A.split_l r (k `US.add` 1sz)) (US.v k) hd2 hd3) in
+            let gs0 = h0 (varraylist pred1 pred2 pred3 pred4 (A.split_l r k) (US.v hd) hd2 hd3 hd4) in
+            let gs1 = h1 (varraylist pred1 pred2 pred3 pred4 (A.split_l r (k `US.add` 1sz)) (US.v k) hd2 hd3 hd4) in
             AL.ptrs_in (US.v k) gs1 ==
             FS.insert (US.v k) (AL.ptrs_in (US.v hd) gs0) /\
             AL.ptrs_in hd2 gs1 == AL.ptrs_in hd2 gs0 /\
             AL.ptrs_in hd3 gs1 == AL.ptrs_in hd3 gs0 /\
+            AL.ptrs_in hd4 gs1 == AL.ptrs_in hd4 gs0 /\
             AL.dataify gs1 == Seq.append (AL.dataify gs0) (Seq.create 1 v)
           )
-  = AL.extend r hd hd2 hd3 k v
+  = AL.extend r hd hd2 hd3 hd4 k v
 
 inline_for_extraction noextract
 let extend1
-  (#pred1 #pred2 #pred3: status -> prop)
+  (#pred1 #pred2 #pred3 #pred4: status -> prop)
   (r:A.array cell)
   (hd:US.t{hd == null_ptr \/ US.v hd < A.length r})
-  (hd2 hd3:Ghost.erased nat)
+  (hd2 hd3 hd4:Ghost.erased nat)
   (k:US.t{US.v k + 1 <= A.length r /\ US.fits (US.v k + 1)})
   (v: status)
   : Steel unit
-          (AL.varraylist pred1 pred2 pred3 (A.split_l r k) (US.v hd) hd2 hd3 `star`
+          (AL.varraylist pred1 pred2 pred3 pred4 (A.split_l r k) (US.v hd) hd2 hd3 hd4 `star`
             A.varray (A.split_l (A.split_r r k) 1sz))
           (fun _ ->
-            AL.varraylist pred1 pred2 pred3 (A.split_l r (k `US.add` 1sz)) (US.v k) hd2 hd3)
+            AL.varraylist pred1 pred2 pred3 pred4 (A.split_l r (k `US.add` 1sz)) (US.v k) hd2 hd3 hd4)
           (requires fun _ ->
             k <> null_ptr /\ pred1 v)
           (ensures fun h0 _ h1 ->
             A.length_fits r;
-            let gs0 = h0 (varraylist pred1 pred2 pred3 (A.split_l r k) (US.v hd) hd2 hd3) in
-            let gs1 = h1 (varraylist pred1 pred2 pred3 (A.split_l r (k `US.add` 1sz)) (US.v k) hd2 hd3) in
+            let gs0 = h0 (varraylist pred1 pred2 pred3 pred4 (A.split_l r k) (US.v hd) hd2 hd3 hd4) in
+            let gs1 = h1 (varraylist pred1 pred2 pred3 pred4 (A.split_l r (k `US.add` 1sz)) (US.v k) hd2 hd3 hd4) in
             AL.ptrs_in (US.v k) gs1 ==
             FS.insert (US.v k) (AL.ptrs_in (US.v hd) gs0) /\
             AL.ptrs_in hd2 gs1 == AL.ptrs_in hd2 gs0 /\
             AL.ptrs_in hd3 gs1 == AL.ptrs_in hd3 gs0 /\
+            AL.ptrs_in hd4 gs1 == AL.ptrs_in hd4 gs0 /\
             AL.dataify gs1 `Seq.equal` Seq.append (AL.dataify gs0) (Seq.create 1 v)
           )
-  = extend r hd hd2 hd3 k v
+  = extend r hd hd2 hd3 hd4 k v
